flake.nix
@@ -12,6 +12,21 @@
         pkgs = import nixpkgs { inherit system; };
         coq = pkgs.coq_8_18;
         coqPackages = pkgs.coqPackages_8_18;
+        coq-nbits = coqPackages.mkCoqDerivation {
+          pname = "coq-nbits";
+          owner = "fmlab-iis";
+          version = "2022-11-28";
+          release = {
+            "2022-11-28" = {
+              rev = "c360c35bd263807d0f960f4edfac713b1257ea80";
+              sha256 = "sha256-eeF1HouyyPxZG8wdEtxQP1daO7taxNVGzMyWv7UkE0k=";
+            };
+          };
+          propagatedBuildInputs = [
+            coqPackages.mathcomp.ssreflect
+            coqPackages.mathcomp.algebra
+          ];
+        };
       in {
         devShells.default = pkgs.mkShell {
           packages =
@@ -19,6 +34,7 @@
               coq
               coqPackages.coq-ext-lib
               coqPackages.equations
+              coq-nbits
 
               coq.ocaml
               coq.ocamlPackages.findlib
